almost working memmove example

dimsum_examples/iris/rec.v
@@ -8,6 +8,388 @@ Set Default Proof Using "Type".
 
 Local Open Scope Z_scope.
 
+
+Section sim.
+  Context {Σ : gFunctors} {EV : Type} `{!dimsumGS Σ}.
+
+  Definition sim_tgt_handler {m_t m_s : mod_trans EV}
+    (σ : m_state m_s) :
+    option EV → ((m_state m_t → iProp Σ) → iProp Σ) → iProp Σ :=
+    λ κ Pσ, (σ ≈{m_s}≈>ₛ (λ κ' σ_s', ⌜κ = κ'⌝ ∗ bi_mono1 Pσ (λ σ_t', σ_t' ⪯{m_t, m_s} σ_s')))%I.
+
+  Lemma sim_tgt_handler_intro m_t m_s σ_t σ_s :
+    σ_t ≈{m_t}≈>ₜ sim_tgt_handler σ_s -∗ σ_t ⪯{m_t, m_s} σ_s.
+  Proof. iIntros "?". by rewrite sim_unfold. Qed.
+
+End sim.
+
+Section link.
+  Context {Σ : gFunctors} {EV : Type} {S : Type} `{!dimsumGS Σ}.
+  Implicit Types (R : seq_product_case → S → EV → seq_product_case → S → EV → bool → Prop).
+
+  Lemma sim_tgt_link_None R m1 m2 s σ1 σ2 Π :
+    ▷ₒ (∀ e p' s' e' ok,
+        ⌜R SPNone s e p' s' e' ok⌝ -∗
+        Π (Some (Incoming, e')) (λ P, P (link_to_case ok p' e', s', σ1, σ2))) -∗
+    (MLFNone, s, σ1, σ2) ≈{link_trans R m1 m2}≈>ₜ Π.
+  Proof.
+    iIntros "HΠ".
+    iApply (sim_tgt_bi_mono1 with "[-]").
+    iApply sim_tgt_state_transform; [done|] => /=.
+    iApply (sim_tgt_map with "[-]").
+    iApply sim_tgt_seq_product_None. iIntros (p) "!>". iIntros (????).
+    inv_all @link_filter.
+    iApply (bi_mono1_intro with "[HΠ]"); [by iApply "HΠ"|] => /=.
+    iIntros (?) "?". iIntros ([[[??]?]?] ?); simplify_eq/=. by repeat case_match; simplify_eq/=.
+  Qed.
+
+  Definition link_tgt_left_handler R {m1 m2 : mod_trans (io_event EV)}
+    (Π : option (io_event EV) → ((link_case EV * S * m_state m1 * m_state m2 → iProp Σ) → iProp Σ) → iProp Σ)
+    (s : S) (σ2 : m_state m2)
+    : option (io_event EV) → ((m_state m1 → iProp Σ) → iProp Σ) → iProp Σ :=
+    λ κ Pσ,
+      match κ with
+            | None => Π None (λ P, Pσ (λ σ1', P (MLFLeft, s, σ1', σ2)))
+            | Some e => ∀ p' s' e' ok, ⌜R SPLeft s e.2 p' s' e' ok⌝ -∗ ⌜e.1 = Outgoing⌝ -∗
+                 Π (if p' is SPNone then Some (Outgoing, e') else None)
+                 (λ P, Pσ (λ σ1', P (link_to_case ok p' e', s', σ1', σ2)))
+            end%I.
+
+  Lemma sim_tgt_link_left R m1 m2 s σ1 σ2 Π :
+    σ1 ≈{m1}≈>ₜ link_tgt_left_handler R Π s σ2 -∗
+    (MLFLeft, s, σ1, σ2) ≈{link_trans R m1 m2}≈>ₜ Π.
+  Proof.
+    iIntros "Hsim".
+    iApply (sim_tgt_bi_mono1 with "[-]").
+    iApply sim_tgt_state_transform; [done|] => /=.
+    iApply (sim_tgt_map with "[-]").
+    iApply sim_tgt_seq_product_left.
+    iApply (sim_tgt_bi_mono2 with "[-]").
+    iApply (sim_tgt_wand with "Hsim").
+    iIntros (κ ?) "Hsim". iIntros (??????). destruct κ; destruct!/=.
+    - inv_all @link_filter.
+      iApply (bi_mono1_intro with "[Hsim]"); [by iApply "Hsim"|].
+      iIntros (?) "HP". iApply (bi_mono1_intro with "HP").
+      iIntros (?) "?". iIntros ([[[??]?]?]?). simplify_eq/=. by repeat case_match; simplify_eq/=.
+    - iApply (bi_mono1_intro with "[Hsim]"); [by iApply "Hsim"|].
+      iIntros (?) "HP". iApply (bi_mono1_intro with "HP").
+      iIntros (?) "?". iIntros ([[[??]?]?]?). simplify_eq/=. done.
+  Qed.
+
+  Lemma sim_tgt_link_left_recv R m1 m2 s σ1 σ2 Π e :
+    (σ1 ≈{m1}≈>ₜ λ κ Pσ,
+      match κ with
+      | None => Π None (λ P, Pσ (λ σ1', P (MLFRecvL e, s, σ1', σ2)))
+      | Some e' => ⌜e' = (Incoming, e)⌝ -∗ Π None (λ P, Pσ (λ σ1', P (MLFLeft, s, σ1', σ2)))
+      end%I) -∗
+    (MLFRecvL e, s, σ1, σ2) ≈{link_trans R m1 m2}≈>ₜ Π.
+  Proof.
+    iIntros "Hsim".
+    iApply (sim_tgt_bi_mono1 with "[-]").
+    iApply sim_tgt_state_transform; [done|] => /=.
+    iApply (sim_tgt_map with "[-]").
+    iApply sim_tgt_seq_product_left.
+    iApply (sim_tgt_bi_mono2 with "[-]").
+    iApply (sim_tgt_wand with "Hsim").
+    iIntros (κ ?) "Hsim". iIntros (??????). destruct κ; destruct!/=.
+    - inv_all @link_filter.
+      iApply (bi_mono1_intro with "[Hsim]"); [by iApply "Hsim"|].
+      iIntros (?) "HP". iApply (bi_mono1_intro with "HP").
+      iIntros (?) "?". iIntros ([[[??]?]?]?). by simplify_eq/=.
+    - iApply (bi_mono1_intro with "[Hsim]"); [by iApply "Hsim"|].
+      iIntros (?) "HP". iApply (bi_mono1_intro with "HP").
+      iIntros (?) "?". iIntros ([[[??]?]?]?). simplify_eq/=. done.
+  Qed.
+
+  Definition link_tgt_right_handler R {m1 m2 : mod_trans (io_event EV)}
+    (Π : option (io_event EV) → ((link_case EV * S * m_state m1 * m_state m2 → iProp Σ) → iProp Σ) → iProp Σ)
+    (s : S) (σ1 : m_state m1)
+    : option (io_event EV) → ((m_state m2 → iProp Σ) → iProp Σ) → iProp Σ :=
+    λ κ Pσ,
+      match κ with
+            | None => Π None (λ P, Pσ (λ σ2', P (MLFRight, s, σ1, σ2')))
+            | Some e => ∀ p' s' e' ok, ⌜R SPRight s e.2 p' s' e' ok⌝ -∗ ⌜e.1 = Outgoing⌝ -∗
+                 Π (if p' is SPNone then Some (Outgoing, e') else None)
+                 (λ P, Pσ (λ σ2', P (link_to_case ok p' e', s', σ1, σ2')))
+            end%I.
+
+  Lemma sim_tgt_link_right R m1 m2 s σ1 σ2 Π :
+    σ2 ≈{m2}≈>ₜ link_tgt_right_handler R Π s σ1 -∗
+    (MLFRight, s, σ1, σ2) ≈{link_trans R m1 m2}≈>ₜ Π.
+  Proof.
+    iIntros "Hsim".
+    iApply (sim_tgt_bi_mono1 with "[-]").
+    iApply sim_tgt_state_transform; [done|] => /=.
+    iApply (sim_tgt_map with "[-]").
+    iApply sim_tgt_seq_product_right.
+    iApply (sim_tgt_bi_mono2 with "[-]").
+    iApply (sim_tgt_wand with "Hsim").
+    iIntros (κ ?) "Hsim". iIntros (??????). destruct κ; destruct!/=.
+    - inv_all @link_filter.
+      iApply (bi_mono1_intro with "[Hsim]"); [by iApply "Hsim"|].
+      iIntros (?) "HP". iApply (bi_mono1_intro with "HP").
+      iIntros (?) "?". iIntros ([[[??]?]?]?). simplify_eq/=. by repeat case_match; simplify_eq/=.
+    - iApply (bi_mono1_intro with "[Hsim]"); [by iApply "Hsim"|].
+      iIntros (?) "HP". iApply (bi_mono1_intro with "HP").
+      iIntros (?) "?". iIntros ([[[??]?]?]?). simplify_eq/=. done.
+  Qed.
+
+  Lemma sim_tgt_link_right_recv R m1 m2 s σ1 σ2 Π e :
+    (σ2 ≈{m2}≈>ₜ λ κ Pσ,
+      match κ with
+      | None => Π None (λ P, Pσ (λ σ2', P (MLFRecvR e, s, σ1, σ2')))
+      | Some e' => ⌜e' = (Incoming, e)⌝ -∗ Π None (λ P, Pσ (λ σ2', P (MLFRight, s, σ1, σ2')))
+      end%I) -∗
+    (MLFRecvR e, s, σ1, σ2) ≈{link_trans R m1 m2}≈>ₜ Π.
+  Proof.
+    iIntros "Hsim".
+    iApply (sim_tgt_bi_mono1 with "[-]").
+    iApply sim_tgt_state_transform; [done|] => /=.
+    iApply (sim_tgt_map with "[-]").
+    iApply sim_tgt_seq_product_right.
+    iApply (sim_tgt_bi_mono2 with "[-]").
+    iApply (sim_tgt_wand with "Hsim").
+    iIntros (κ ?) "Hsim". iIntros (??????). destruct κ; destruct!/=.
+    - inv_all @link_filter.
+      iApply (bi_mono1_intro with "[Hsim]"); [by iApply "Hsim"|].
+      iIntros (?) "HP". iApply (bi_mono1_intro with "HP").
+      iIntros (?) "?". iIntros ([[[??]?]?]?). by simplify_eq/=.
+    - iApply (bi_mono1_intro with "[Hsim]"); [by iApply "Hsim"|].
+      iIntros (?) "HP". iApply (bi_mono1_intro with "HP").
+      iIntros (?) "?". iIntros ([[[??]?]?]?). simplify_eq/=. done.
+  Qed.
+End link.
+
+
+Program Definition spec_mod_lang {Σ} (EV S : Type) (state_interp : S → iProp Σ)  : mod_lang EV Σ := {|
+  mexpr := spec EV S void;
+  mectx := unit;
+  mfill _ := id;
+  mcomp_ectx _ _:= tt;
+  mtrans := spec_trans EV S;
+  mexpr_rel σ t := σ.1 ≡ t;
+  mstate_interp σ := state_interp σ.2;
+|}.
+Next Obligation. done. Qed.
+
+Definition spec_mod_lang_unit {Σ} (EV : Type) : mod_lang EV Σ :=
+  spec_mod_lang EV unit (λ _, True%I).
+
+Section spec.
+  Context `{!dimsumGS Σ} {EV S : Type} {state_interp : S → iProp Σ}.
+
+  Global Instance sim_tgt_expr_spec_proper :
+    Proper ((≡) ==> (=) ==> (=) ==> (⊣⊢)) (sim_tgt_expr (Λ:=spec_mod_lang EV S state_interp)).
+  Proof.
+    move => ?? ? ?? -> ?? ->.
+    Local Transparent sim_tgt_expr.
+    Local Typeclasses Transparent sim_tgt_expr.
+    iSplit; iIntros "HP" (?) "?"; iIntros (??); simplify_eq/=; iApply ("HP" with "[$]"); iPureIntro => /=.
+    all: by etrans; [done|].
+    Unshelve. all: exact tt.
+  Qed.
+
+  Global Instance sim_src_expr_spec_proper :
+    Proper ((≡) ==> (=) ==> (=) ==> (⊣⊢)) (sim_src_expr (Λ:=spec_mod_lang EV S state_interp)).
+  Proof.
+    move => ?? ? ?? -> ?? ->.
+    Local Transparent sim_src_expr.
+    Local Typeclasses Transparent sim_src_expr.
+    iSplit; iIntros "HP" (?) "?"; iIntros (??); simplify_eq/=; iApply ("HP" with "[$]"); iPureIntro => /=.
+    all: by etrans; [done|].
+    Unshelve. all: exact tt.
+  Qed.
+
+  Let X := (spec_mod_lang EV _ state_interp).
+  Local Canonical Structure X.
+
+  Lemma sim_tgt_TVis k Π Φ e :
+    (▷ₒ Π (Some e) (λ P, (∀ σ, σ ⤇ₜ (λ Π, TGT k tt [{ Π }] {{ Φ }}) -∗ P σ))) -∗
+    TGT (Spec.bind (TVis e) k) [{ Π }] {{ Φ }}.
+  Proof.
+    iIntros "Hsim". rewrite unfold_bind/=. setoid_rewrite unfold_bind; simpl.
+    iApply sim_tgt_expr_bi_mono.
+    iApply sim_tgt_expr_step. iIntros (?[??]?? Heq Hstep) "Hs". simplify_eq/=. iModIntro.
+    inv/= Hstep.
+    all: revert select (_ ≡ _); rewrite Heq; try by move => /spec_equiv_inv.
+    move => /spec_equiv_inv //= [? Heq2]. simplify_eq/=.
+    iModIntro. iApply (bi_mono1_intro with "Hsim"). iIntros (?) "Hσ".
+    iSplit!. iIntros "Htgt". iApply "Hσ". by iApply "Htgt".
+  Qed.
+
+  Lemma sim_src_TVis k Π Φ e :
+    (∀ σ, σ ⤇ₛ (λ Π, SRC k tt [{ Π }] {{ Φ }}) -∗ Π (Some e) σ) -∗
+    SRC (Spec.bind (TVis e) k) [{ Π }] {{ Φ }}.
+  Proof.
+    iIntros "Hsim". rewrite unfold_bind/=. setoid_rewrite unfold_bind; simpl.
+    iApply sim_src_expr_step. iIntros (?[??]?) "?". simplify_eq/=. iModIntro.
+    iExists _, _. iSplit. { iPureIntro. by econs. }
+    iIntros ([??] ?) "!> HΦ". simplify_eq.
+    iApply "Hsim". iIntros (?) "?". by iApply ("HΦ" with "[//] [$]").
+  Qed.
+
+  Lemma sim_tgt_TAll {T} x k Π Φ :
+    (▷ₒ TGT (k x) [{ Π }] {{ Φ }}) -∗
+    TGT (Spec.bind (TAll T) k) [{ Π }] {{ Φ }}.
+  Proof.
+    iIntros "Hsim". rewrite unfold_bind/=. setoid_rewrite unfold_bind; simpl.
+    iApply sim_tgt_expr_step_None. iIntros (?[??]?? Heq Hstep) "Hs". simplify_eq/=. iModIntro.
+    inv/= Hstep.
+    all: revert select (_ ≡ _); rewrite Heq; try by move => /spec_equiv_inv.
+    move => /spec_equiv_inv //= [? Heq2]. simplify_eq/=.
+    iModIntro. rewrite Heq2. iSplit!. iFrame.
+  Qed.
+
+  Lemma sim_src_TAll {T} k Π Φ :
+    (∀ x, SRC (k x) [{ Π }] {{ Φ }}) -∗
+    SRC (Spec.bind (TAll T) k) [{ Π }] {{ Φ }}.
+  Proof.
+    iIntros "Hsim". rewrite unfold_bind/=. setoid_rewrite unfold_bind; simpl.
+    iApply sim_src_expr_step_None. iIntros (?[??]?) "?". simplify_eq/=. iModIntro.
+    iExists _. iSplit. { iPureIntro. by econs. }
+    iIntros ([??] [??]) "!>". simplify_eq. iSplit!. iFrame. iApply "Hsim".
+  Qed.
+
+  Lemma sim_tgt_TExist {T} k Π Φ :
+    (∀ x, ▷ₒ TGT (k x) [{ Π }] {{ Φ }}) -∗
+    TGT (Spec.bind (TExist T) k) [{ Π }] {{ Φ }}.
+  Proof.
+    iIntros "Hsim". rewrite unfold_bind/=. setoid_rewrite unfold_bind; simpl.
+    iApply sim_tgt_expr_step_None. iIntros (?[??]?? Heq Hstep) "Hs". simplify_eq/=. iModIntro.
+    inv/= Hstep.
+    all: revert select (_ ≡ _); rewrite Heq; try by move => /spec_equiv_inv.
+    move => /spec_equiv_inv //= [? Heq2]. simplify_eq/=. iSpecialize ("Hsim" $! _).
+    iModIntro. rewrite Heq2. iSplit!. iFrame.
+  Qed.
+
+  Lemma sim_src_TExist {T} x k Π Φ :
+    SRC (k x) [{ Π }] {{ Φ }} -∗
+    SRC (Spec.bind (TExist T) k) [{ Π }] {{ Φ }}.
+  Proof.
+    iIntros "Hsim". rewrite unfold_bind/=. setoid_rewrite unfold_bind; simpl.
+    iApply sim_src_expr_step_None. iIntros (?[??]?) "?". simplify_eq/=. iModIntro.
+    iExists _. iSplit. { iPureIntro. by econs. }
+    iIntros ([??] ?) "!>". simplify_eq. iSplit!. iFrame.
+  Qed.
+
+  Lemma sim_tgt_TNb T (k : T → _) Π Φ :
+    ⊢ TGT (Spec.bind TNb k) [{ Π }] {{ Φ }}.
+  Proof.
+    rewrite unfold_bind/=. setoid_rewrite unfold_bind; simpl.
+    iApply sim_tgt_expr_step_None. iIntros (?[??]?? Heq Hstep) "Hs". simplify_eq/=. iModIntro.
+    inv/= Hstep.
+    all: revert select (_ ≡ _); rewrite Heq; try by move => /spec_equiv_inv.
+    move => /spec_equiv_inv //= [? Heq2]. simplify_eq/=. destruct_all void.
+  Qed.
+
+  Lemma sim_tgt_TNb_end Π Φ :
+    ⊢ TGT TNb [{ Π }] {{ Φ }}.
+  Proof.
+    iApply sim_tgt_expr_step_None. iIntros (?[??]?? Heq Hstep) "Hs". simplify_eq/=. iModIntro.
+    inv/= Hstep.
+    all: revert select (_ ≡ _); rewrite Heq; try by move => /spec_equiv_inv.
+    move => /spec_equiv_inv //= [? Heq2]. simplify_eq/=. destruct_all void.
+  Qed.
+
+  Lemma sim_src_TUb T (k : T → _) Π Φ :
+    ⊢ SRC (Spec.bind TUb k) [{ Π }] {{ Φ }}.
+  Proof.
+    rewrite unfold_bind/=. setoid_rewrite unfold_bind; simpl.
+    iApply sim_src_expr_step_None. iIntros (?[??]?) "?". simplify_eq/=. iModIntro.
+    iExists _. iSplit. { iPureIntro. by econs. }
+    iIntros ([??] [??]) "!>". destruct_all void.
+  Qed.
+
+  Lemma sim_src_TUb_end Π Φ :
+    ⊢ SRC (TUb) [{ Π }] {{ Φ }}.
+  Proof.
+    iApply sim_src_expr_step_None. iIntros (?[??]?) "?". simplify_eq/=. iModIntro.
+    iExists _. iSplit. { iPureIntro. by econs. }
+    iIntros ([??] [??]) "!>". destruct_all void.
+  Qed.
+
+  Lemma sim_tgt_TAssume k Π Φ (P : Prop) :
+    P →
+    (▷ₒ TGT (k tt) [{ Π }] {{ Φ }}) -∗
+    TGT (Spec.bind (TAssume P) k) [{ Π }] {{ Φ }}.
+  Proof.
+    iIntros (?) "Hsim". rewrite unfold_bind/=. setoid_rewrite unfold_bind; simpl.
+    iApply sim_tgt_expr_step_None. iIntros (?[??]?? Heq Hstep) "Hs". simplify_eq/=. iModIntro.
+    inv/= Hstep.
+    all: revert select (_ ≡ _); rewrite Heq; try by move => /spec_equiv_inv.
+    move => /spec_equiv_inv //= [? Heq2]. simplify_eq/=.
+    iModIntro. rewrite Heq2. iSplit!. iFrame.
+    Unshelve. done.
+  Qed.
+
+  Lemma sim_src_TAssume k Π Φ P :
+    (⌜P⌝ -∗ SRC (k tt) [{ Π }] {{ Φ }}) -∗
+    SRC (Spec.bind (TAssume P) k) [{ Π }] {{ Φ }}.
+  Proof.
+    iIntros "Hsim". rewrite unfold_bind/=. setoid_rewrite unfold_bind; simpl.
+    iApply sim_src_expr_step_None. iIntros (?[??]?) "?". simplify_eq/=. iModIntro.
+    iExists _. iSplit. { iPureIntro. by econs. }
+    iIntros ([??] [??]) "!>". simplify_eq. iSplit!. iFrame. by iApply "Hsim".
+  Qed.
+
+  Lemma sim_tgt_TAssert k Π Φ (P : Prop) :
+    (⌜P⌝ -∗ ▷ₒ TGT (k tt) [{ Π }] {{ Φ }}) -∗
+    TGT (Spec.bind (TAssert P) k) [{ Π }] {{ Φ }}.
+  Proof.
+    iIntros "Hsim". rewrite unfold_bind/=. setoid_rewrite unfold_bind; simpl.
+    iApply sim_tgt_expr_step_None. iIntros (?[??]?? Heq Hstep) "Hs". simplify_eq/=. iModIntro.
+    inv/= Hstep.
+    all: revert select (_ ≡ _); rewrite Heq; try by move => /spec_equiv_inv.
+    move => /spec_equiv_inv //= [? Heq2]. simplify_eq/=. iSpecialize ("Hsim" with "[//]").
+    iModIntro. rewrite Heq2. iSplit!. iFrame.
+  Qed.
+
+  Lemma sim_src_TAssert k Π Φ (P : Prop) :
+    P →
+    SRC (k tt) [{ Π }] {{ Φ }} -∗
+    SRC (Spec.bind (TAssert P) k) [{ Π }] {{ Φ }}.
+  Proof.
+    iIntros (?) "Hsim". rewrite unfold_bind/=. setoid_rewrite unfold_bind; simpl.
+    iApply sim_src_expr_step_None. iIntros (?[??]?) "?". simplify_eq/=. iModIntro.
+    iExists _. iSplit. { iPureIntro. by econs. }
+    iIntros ([??] ?) "!>". simplify_eq. iSplit!. iFrame.
+    Unshelve. done.
+  Qed.
+
+  Lemma sim_tgt_TAssumeOpt {T} o (x : T) k Π Φ :
+    o = Some x →
+    TGT k x [{ Π }] {{ Φ }} -∗
+    TGT (Spec.bind (TAssumeOpt o) k) [{ Π }] {{ Φ }}.
+  Proof. iIntros (->) "Hsim". simpl. by rewrite unfold_bind/=. Qed.
+
+  Lemma sim_src_TAssumeOpt {T} (o : option T) k Π Φ :
+    (∀ x, ⌜o = Some x⌝ -∗ SRC k x [{ Π }] {{ Φ }}) -∗
+    SRC (Spec.bind (TAssumeOpt o) k) [{ Π }] {{ Φ }}.
+  Proof.
+    iIntros "Hsim".
+    destruct o => /=.
+    - rewrite unfold_bind/=. by iApply "Hsim".
+    - iApply sim_src_TUb.
+  Qed.
+
+  Lemma sim_tgt_TAssertOpt {T} (o : option T) k Π Φ :
+    (∀ x, ⌜o = Some x⌝ -∗ TGT k x [{ Π }] {{ Φ }}) -∗
+    TGT (Spec.bind (TAssertOpt o) k) [{ Π }] {{ Φ }}.
+  Proof.
+    iIntros "Hsim".
+    destruct o => /=.
+    - rewrite unfold_bind/=. by iApply "Hsim".
+    - iApply sim_tgt_TNb.
+  Qed.
+
+  Lemma sim_src_TAssertOpt {T} o (x : T) k Π Φ :
+    o = Some x →
+    SRC k x [{ Π }] {{ Φ }} -∗
+    SRC (Spec.bind (TAssertOpt o) k) [{ Π }] {{ Φ }}.
+  Proof. iIntros (->) "Hsim". simpl. by rewrite unfold_bind/=. Qed.
+End spec.
+
+
 Definition fnsUR : cmra :=
   agreeR (gmapO string (leibnizO fndef)).
 
@@ -160,68 +542,6 @@ Next Obligation. move => ???? [??]/=. by rewrite /expr_heap_fill/= expr_fill_app
 Section lifting.
   Context `{!dimsumGS Σ} `{!recGS Σ}.
 
-  Lemma sim_tgt_rec_BinOp Π Φ v1 v2 v3 op :
-    eval_binop op v1 v2 = Some v3 →
-    (▷ₒ Φ (Val v3 @ -) Π) -∗
-    TGT BinOp (Val v1) op (Val v2) @ - [{ Π }] {{ Φ }}.
-  Proof.
-    iIntros (Hop) "HΦ".
-    iApply sim_tgt_expr_step_None => /=. iIntros (? [e' h fns] ?? [??] Hp) "[Hh [Ha Hfns]]". simplify_eq/=.
-    exploit prim_step_inv_head; [done|..].
-    { apply sub_redexes_are_values_item; case; naive_solver. }
-    { done. }
-    move => [? [Hstep ?]]. inv Hstep.
-    do 2 iModIntro. iExists _, (_ @ -). iSplit!. iFrame.
-    by iApply sim_tgt_expr_stop2.
-  Qed.
-
-  Lemma sim_tgt_rec_If Π Φ (b : bool) e1 e2 :
-    (▷ₒ TGT (if b then e1 else e2) @ - [{ Π }] {{ Φ }}) -∗
-    TGT If (Val (ValBool b)) e1 e2 @ - [{ Π }] {{ Φ }}.
-  Proof.
-    iIntros "HΦ".
-    iApply sim_tgt_expr_step_None => /=. iIntros (? [e' h fns] ?? [??] Hp) "[Hh [Ha Hfns]]". simplify_eq/=.
-    exploit prim_step_inv_head; [done|..].
-    { apply sub_redexes_are_values_item; case; naive_solver. }
-    { done. }
-    move => [? [Hstep ?]]. inv Hstep.
-    do 2 iModIntro. iExists _, (_ @ -). iSplit!. iFrame.
-  Qed.
-
-  Lemma sim_tgt_rec_AllocA e Π Φ vs :
-    Forall (λ z, 0 < z) vs.*2 →
-    (∀ ls, ([∗ list] l;n∈ls; vs.*2, [∗ list] o∈seqZ 0 n, (l +ₗ o) ↦ 0) -∗
-     ▷ₒ TGT subst_l vs.*1 (ValLoc <$> ls) e @ - [{ Π }] {{ e', Π',
-     ∃ v, ⌜e' = Val v @ -⌝ ∗ ([∗ list] l;n∈ls; vs.*2, [∗ list] o∈seqZ 0 n, ∃ v, (l +ₗ o) ↦ v) ∗ Φ e' Π' }}) -∗
-    TGT AllocA vs e @ - [{ Π }] {{ Φ }}.
-  Proof.
-    iIntros (Hall) "HΦ".
-    iApply sim_tgt_expr_step_None => /=. iIntros (? [e' h fns] ?? [??] Hp) "[Hh [Ha Hfns]]". simplify_eq/=.
-    exploit prim_step_inv_head; [done|..].
-    { apply sub_redexes_are_values_item; case; naive_solver. }
-    { done. }
-    move => [? [Hstep ?]]. inv Hstep.
-    do 2 iModIntro. iExists _, (_ @ -). iSplit!. iFrame. simpl.
-  Admitted.
-
-  Lemma sim_tgt_rec_Call_internal f fn es Π Φ vs `{!AsVals es vs None} :
-    length vs = length (fd_args fn) →
-    f ↪ Some fn -∗
-    (▷ₒ TGT AllocA fn.(fd_vars) (subst_l fn.(fd_args) vs fn.(fd_body)) @ - [{ Π }] {{ Φ }}) -∗
-    TGT Call f es @ - [{ Π }] {{ Φ }}.
-  Proof.
-    destruct AsVals0. iIntros (?) "Hfn HΦ".
-    iApply sim_tgt_expr_step_None => /=. iIntros (? [e h fns] ?? [??] Hp) "[Hh [Ha Hfns]]". simplify_eq/=.
-    iDestruct (rec_fn_lookup with "[$] [$]") as %?.
-    rewrite right_id_L in Hp.
-    exploit prim_step_inv_head; [done|..].
-    { apply sub_redexes_are_values_item; case; try naive_solver.
-      move => /= ??? e' [_ Heq]. by apply: list_expr_val_inv. }
-    { done. }
-    move => [? [Hstep ?]]. inv Hstep.
-    do 2 iModIntro. iExists _, (_ @ -). iSplit!. iFrame.
-  Qed.
-
   Lemma sim_tgt_rec_Waiting fns h Π Φ (b : bool) :
     rec_fn_auth fns -∗
     (rec_mapsto_auth (h_heap h) -∗
@@ -258,66 +578,378 @@ Section lifting.
       iSplit!. iIntros "Hc". iApply "Htgt". iIntros "??".
       iApply "Hc"; [done|]. iFrame.
   Qed.
+
+  Lemma sim_tgt_rec_ReturnExt v Π Φ (b : bool) :
+    (∀ h,
+     ▷ₒ Π (Some (Outgoing, ERReturn v h)) (λ P,
+         ∀ σ,
+           (σ ⤇ₜ λ Π', TGT Waiting b @ h [{ Π' }] {{ Φ }}) -∗
+           P σ)) -∗
+    TGT ReturnExt b (Val v) @ - [{ Π }] {{ Φ }}.
+  Proof.
+    iIntros "HΦ".
+    iApply sim_tgt_expr_bi_mono.
+    iApply sim_tgt_expr_step => /=. iIntros (? [e h0 fns0] ?? [??] Hp) "[Hh [Ha Hfns']]". simplify_eq/=.
+    exploit prim_step_inv_head; [done|..].
+    { apply sub_redexes_are_values_item; case; naive_solver. }
+    { done. }
+    move => [? [Hstep ?]]. inv Hstep.
+    iSpecialize ("HΦ" $! _). do 2 iModIntro. iApply (bi_mono1_intro with "HΦ").
+    iIntros (?) "Htgt". iSplit!. iIntros "Hc". iApply "Htgt".
+    iApply "Hc"; [done|]. iFrame.
+  Qed.
+
+  Lemma sim_tgt_rec_Call_internal f fn es Π Φ vs `{!AsVals es vs None} :
+    length vs = length (fd_args fn) →
+    f ↪ Some fn -∗
+    (▷ₒ TGT AllocA fn.(fd_vars) (subst_l fn.(fd_args) vs fn.(fd_body)) @ - [{ Π }] {{ Φ }}) -∗
+    TGT Call f es @ - [{ Π }] {{ Φ }}.
+  Proof.
+    destruct AsVals0. iIntros (?) "Hfn HΦ".
+    iApply sim_tgt_expr_step_None => /=. iIntros (? [e h fns] ?? [??] Hp) "[Hh [Ha Hfns]]". simplify_eq/=.
+    iDestruct (rec_fn_lookup with "[$] [$]") as %?.
+    rewrite right_id_L in Hp.
+    exploit prim_step_inv_head; [done|..].
+    { apply sub_redexes_are_values_item; case; try naive_solver.
+      move => /= ??? e' [_ Heq]. by apply: list_expr_val_inv. }
+    { done. }
+    move => [? [Hstep ?]]. inv Hstep.
+    do 2 iModIntro. iExists _, (_ @ -). iSplit!. iFrame.
+  Qed.
+
+  Lemma sim_tgt_rec_Call_external f es Π Φ vs `{!AsVals es vs None} :
+    f ↪ None -∗
+    (∀ h,
+     ▷ₒ Π (Some (Outgoing, ERCall f vs h)) (λ P,
+         ∀ σ,
+           (σ ⤇ₜ λ Π', TGT Waiting true @ h [{ Π' }] {{ Φ }}) -∗
+           P σ)) -∗
+    TGT Call f es @ - [{ Π }] {{ Φ }}.
+  Proof.
+    destruct AsVals0. iIntros "Hfn HΦ".
+    iApply sim_tgt_expr_bi_mono.
+    iApply sim_tgt_expr_step => /=. iIntros (? [e h0 fns0] ?? [??] Hp) "[Hh [Ha Hfns']]". simplify_eq/=.
+    iDestruct (rec_fn_lookup with "[$] [$]") as %?.
+    rewrite right_id_L in Hp.
+    exploit prim_step_inv_head; [done|..].
+    { apply sub_redexes_are_values_item; case; try naive_solver.
+      move => /= ??? e' [_ Heq]. by apply: list_expr_val_inv. }
+    { done. }
+    move => [? [Hstep ?]]. inv Hstep.
+    iSpecialize ("HΦ" $! _). do 2 iModIntro. iApply (bi_mono1_intro with "HΦ").
+    iIntros (?) "Htgt". iSplit!. iIntros "Hc". iApply "Htgt".
+    iApply "Hc"; [done|]. iFrame.
+  Qed.
+
+  Lemma sim_tgt_rec_BinOp Π Φ v1 v2 v3 op :
+    eval_binop op v1 v2 = Some v3 →
+    (▷ₒ Φ (Val v3 @ -) Π) -∗
+    TGT BinOp (Val v1) op (Val v2) @ - [{ Π }] {{ Φ }}.
+  Proof.
+    iIntros (Hop) "HΦ".
+    iApply sim_tgt_expr_step_None => /=. iIntros (? [e' h fns] ?? [??] Hp) "[Hh [Ha Hfns]]". simplify_eq/=.
+    exploit prim_step_inv_head; [done|..].
+    { apply sub_redexes_are_values_item; case; naive_solver. }
+    { done. }
+    move => [? [Hstep ?]]. inv Hstep.
+    do 2 iModIntro. iExists _, (_ @ -). iSplit!. iFrame.
+    by iApply sim_tgt_expr_stop2.
+  Qed.
+
+  Lemma sim_tgt_rec_Load Π Φ l v :
+    l ↦ v -∗
+    (l ↦ v -∗ ▷ₒ Φ (Val v @ -) Π) -∗
+    TGT Load (Val (ValLoc l)) @ - [{ Π }] {{ Φ }}.
+  Proof.
+    iIntros "Hl HΦ".
+    iApply sim_tgt_expr_step_None => /=. iIntros (? [e' h fns] ?? [??] Hp) "[Hh [Ha Hfns]]". simplify_eq/=.
+    exploit prim_step_inv_head; [done|..].
+    { apply sub_redexes_are_values_item; case; naive_solver. }
+    { done. }
+    move => [? [Hstep ?]]. inv Hstep.
+    iSpecialize ("HΦ" with "[$]").
+    do 2 iModIntro. iExists _, (_ @ -). iSplit!. admit.
+    iFrame. by iApply sim_tgt_expr_stop2.
+  Admitted.
+
+  Lemma sim_tgt_rec_Store Π Φ l v v' :
+    l ↦ v -∗
+    (l ↦ v' -∗ ▷ₒ Φ (Val 0 @ -) Π) -∗
+    TGT Store (Val (ValLoc l)) (Val v') @ - [{ Π }] {{ Φ }}.
+  Proof.
+    iIntros "Hl HΦ".
+    iApply sim_tgt_expr_step_None => /=. iIntros (? [e' h fns] ?? [??] Hp) "[Hh [Ha Hfns]]". simplify_eq/=.
+    exploit prim_step_inv_head; [done|..].
+    { apply sub_redexes_are_values_item; case; naive_solver. }
+    { done. }
+    move => [? [Hstep ?]]. inv Hstep.
+    do 2 iModIntro. iExists _, (_ @ -). iSplit!. admit.
+    iFrame => /=.
+  Admitted.
+
+  Lemma sim_tgt_rec_AllocA e Π Φ vs :
+    Forall (λ z, 0 < z) vs.*2 →
+    (∀ ls, ([∗ list] l;n∈ls; vs.*2, [∗ list] o∈seqZ 0 n, (l +ₗ o) ↦ 0) -∗
+     ▷ₒ TGT subst_l vs.*1 (ValLoc <$> ls) e @ - [{ Π }] {{ e', Π',
+     ∃ v, ⌜e' = Val v @ -⌝ ∗ ([∗ list] l;n∈ls; vs.*2, [∗ list] o∈seqZ 0 n, ∃ v, (l +ₗ o) ↦ v) ∗ Φ e' Π' }}) -∗
+    TGT AllocA vs e @ - [{ Π }] {{ Φ }}.
+  Proof.
+    iIntros (Hall) "HΦ".
+    iApply sim_tgt_expr_step_None => /=. iIntros (? [e' h fns] ?? [??] Hp) "[Hh [Ha Hfns]]". simplify_eq/=.
+    exploit prim_step_inv_head; [done|..].
+    { apply sub_redexes_are_values_item; case; naive_solver. }
+    { done. }
+    move => [? [Hstep ?]]. inv Hstep.
+    do 2 iModIntro. iExists _, (_ @ -). iSplit!. iFrame. simpl.
+  Admitted.
+
+  Lemma sim_tgt_rec_LetE Π Φ s v e :
+    (▷ₒ TGT (subst s v e) @ - [{ Π }] {{ Φ }}) -∗
+    TGT LetE s (Val v) e @ - [{ Π }] {{ Φ }}.
+  Proof.
+    iIntros "HΦ".
+    iApply sim_tgt_expr_step_None => /=. iIntros (? [e' h fns] ?? [??] Hp) "[Hh [Ha Hfns]]". simplify_eq/=.
+    exploit prim_step_inv_head; [done|..].
+    { apply sub_redexes_are_values_item; case; naive_solver. }
+    { done. }
+    move => [? [Hstep ?]]. inv Hstep.
+    do 2 iModIntro. iExists _, (_ @ -). iSplit!. iFrame.
+  Qed.
+
+  Lemma sim_tgt_rec_If Π Φ (b : bool) e1 e2 :
+    (▷ₒ TGT (if b then e1 else e2) @ - [{ Π }] {{ Φ }}) -∗
+    TGT If (Val (ValBool b)) e1 e2 @ - [{ Π }] {{ Φ }}.
+  Proof.
+    iIntros "HΦ".
+    iApply sim_tgt_expr_step_None => /=. iIntros (? [e' h fns] ?? [??] Hp) "[Hh [Ha Hfns]]". simplify_eq/=.
+    exploit prim_step_inv_head; [done|..].
+    { apply sub_redexes_are_values_item; case; naive_solver. }
+    { done. }
+    move => [? [Hstep ?]]. inv Hstep.
+    do 2 iModIntro. iExists _, (_ @ -). iSplit!. iFrame.
+  Qed.
+
 End lifting.
 
 Section memmove.
   Context `{!dimsumGS Σ} `{!recGS Σ}.
 
-  Lemma sim_memcpy Π Φ d d' s' s n o hvs :
-    n = Z.of_nat (length hvs) →
+
+  Local Definition array (l : loc) (vs : list val) : gmap loc val :=
+    (kmap (λ i, l +ₗ i) (map_seqZ 0 vs)).
+
+  Lemma loc_eq (l1 l2 : loc) :
+    l1 = l2 ↔ l1.1 = l2.1 ∧ l1.2 = l2.2.
+  Proof. destruct l1, l2; naive_solver. Qed.
+
+  Lemma array_nil l :
+    array l [] = ∅.
+  Proof. rewrite /array/=. apply kmap_empty. Qed.
+  Lemma array_cons l v vs :
+    array l (v::vs) = <[l:=v]> $ array (l +ₗ 1) vs.
+  Proof.
+    rewrite /array/= kmap_insert offset_loc_0. f_equal.
+    apply map_eq => ?. apply option_eq => ?.
+    rewrite !lookup_kmap_Some. setoid_rewrite lookup_map_seqZ_Some.
+    split => -[i [? [? <-]]]; simplify_eq.
+    - eexists (Z.pred i). split!; [|lia|f_equal; lia].
+      unfold offset_loc. destruct l => /=. f_equal. lia.
+    - eexists (Z.succ i). split!; [|lia|f_equal; lia].
+      unfold offset_loc. destruct l => /=. f_equal. lia.
+  Qed.
+
+  Lemma array_app l vs1 vs2 :
+    array l (vs1 ++ vs2) = array l vs1 ∪ array (l +ₗ length vs1) vs2.
+  Proof.
+    elim: vs1 l. { move => ?/=. by rewrite array_nil offset_loc_0 left_id_L. }
+    move => v vs1 IH l /=. rewrite !array_cons -insert_union_l.
+    rewrite IH. do 3 f_equal. apply loc_eq. split!. lia.
+  Qed.
+
+  Lemma array_insert l1 l2 v vs :
+    l1.1 = l2.1 →
+    l2.2 ≤ l1.2 < l2.2 + length vs →
+    <[l1:=v]> $ array l2 vs = array l2 (<[Z.to_nat (l1.2 - l2.2):=v]>vs).
+  Proof.
+    move => ??. have {1} -> : l1 = l2 +ₗ Z.to_nat (l1.2 - l2.2).
+    { unfold offset_loc. destruct l1, l2; simplify_eq/=. f_equal. lia. }
+    rewrite /array/= map_seqZ_insert. 2: lia.
+    by rewrite kmap_insert.
+  Qed.
+
+  Lemma array_lookup_None l l' vs :
+    array l vs !! l' = None ↔ (l.1 = l'.1 → l'.2 < l.2 ∨ l.2 + length vs ≤ l'.2).
+  Proof.
+    rewrite /array.
+    rewrite lookup_kmap_None.
+    setoid_rewrite lookup_map_seqZ_None.
+    split.
+    - move => Hi Heq.
+      exploit (Hi (l'.2 - l.2)). { unfold offset_loc. destruct l, l'; simplify_eq/=. f_equal. lia. }
+      lia.
+    - move => Hi ??. simplify_eq/=. lia.
+  Qed.
+
+  Lemma sim_memcpy Π Φ d d' s' s n o hvss hvsd :
+    n = Z.of_nat (length hvss) →
+    length hvss = length hvsd →
     o = 1 ∨ o = -1 →
     d' = (if bool_decide (o = 1) then d else d +ₗ (- n + 1)) →
     s' = (if bool_decide (o = 1) then s else s +ₗ (- n + 1)) →
     (if bool_decide (o = 1) then d.1 = s.1 → d.2 ≤ s.2 else d.1 = s.1 → s.2 ≤ d.2) →
     "memcpy" ↪ Some memcpy_rec -∗
-    ([∗ list] i↦v∈hvs, (s' +ₗ i) ↦ v) -∗
-    ([∗ list] i↦_∈hvs, ∃ v, (d' +ₗ i) ↦ v) -∗
-    (([∗ list] i↦v∈hvs, (s' +ₗ i) ↦ v) -∗ ([∗ list] i↦v∈hvs, (d' +ₗ i) ↦ v) -∗ Φ (Val 0 @ -) Π) -∗
+    ([∗ map] l↦v∈array s' hvss ∪ array d' hvsd, l ↦ v) -∗
+    (([∗ map] l↦v∈array d' hvss ∪ array s' hvss, l ↦ v) -∗
+     Φ (Val 0 @ -) Π) -∗
     TGT Call "memcpy" [Val (ValLoc d); Val $ ValLoc s; Val $ ValNum n; Val $ ValNum o] @ - [{ Π }] {{ Φ }}.
   Proof.
-    iIntros (Hn Ho Hd' Hs' Hle) "#Hf Hs Hd HΦ".
+    iIntros (Hn Hlen Ho Hd' Hs' Hle) "#Hf Hm HΦ".
     iApply sim_tgt_expr_ctx. iIntros "#?".
-    iRevert (d d' s s' n hvs Hn Hd' Hs' Hle) "Hs Hd HΦ".
+    iRevert (hvss hvsd d d' s s' n Φ Hn Hlen Hd' Hs' Hle) "Hm HΦ".
     iApply ord_loeb; [done|].
-    iIntros "!> #IH" (d d' s s' n hvs Hn Hd' Hs' Hle) "Hs Hd HΦ". simplify_eq.
-    iApply (sim_tgt_rec_Call_internal with "Hf"); [done|].
-    (* TODO: ask Robbert whether one can get rid of the following dance: *)
-    iDestruct (ord_later_pers with "IH") as "-#IH2". iClear "IH".
-    iModIntro => /=. iDestruct "IH2" as "#IH".
+    iIntros "!> #IH" (hvss hvsd d d' s s' n Φ Hn Hlen Hd' Hs' Hle) "Hm HΦ". simplify_eq.
+    iApply (sim_tgt_rec_Call_internal with "Hf"); [done|]. iModIntro => /=.
     iApply sim_tgt_rec_AllocA; [econs|] => /=. iIntros (?) "?". destruct ls => //. iModIntro.
     iApply (sim_tgt_expr_bind [IfCtx _ _] (_ @ -) with "[-]") => /=.
     iApply sim_tgt_rec_BinOp; [done|]. iModIntro => /=.
     iApply sim_tgt_rec_If. iModIntro => /=. case_bool_decide (0 < _).
-    2: { destruct hvs => //. iApply sim_tgt_expr_stop2. iSplit!. by iApply "HΦ". }
+    2: { destruct hvss, hvsd => //. iApply sim_tgt_expr_stop2. iSplit!. iApply "HΦ".
+         by rewrite /array !kmap_empty. }
     iApply (sim_tgt_expr_bind [LetECtx _ _] (_ @ -) with "[-]") => /=.
     iApply (sim_tgt_expr_bind [StoreRCtx _] (_ @ -) with "[-]") => /=.
-    admit.
+    destruct Ho; simplify_eq; case_bool_decide => //.
+    - destruct hvss as [|v hvss]; [done|] => /=.
+      destruct hvsd as [|vd hvsd]; [done|] => /=.
+      rewrite !array_cons.
+      iDestruct (big_sepM_lookup_acc _ _ s v with "[$]") as "[Hsv Hm]". { by simplify_map_eq. }
+      iApply (sim_tgt_rec_Load with "Hsv"). iIntros "Hsv !>" => /=.
+      iDestruct ("Hm" with "[$]") as "Hm".
+      have [? Hx]: is_Some ((<[s:=v]> (array (s +ₗ 1) hvss) ∪ <[d:=vd]> (array (d +ₗ 1) hvsd)) !! d).
+      { apply lookup_union_is_Some. simplify_map_eq. naive_solver. }
+      rewrite (big_sepM_delete _ _ _ _ Hx).
+      iDestruct "Hm" as "[Hdv Hm]".
+      iApply (sim_tgt_rec_Store with "Hdv"). iIntros "Hdv !>" => /=.
+      iApply (sim_tgt_rec_LetE). iIntros "!>" => /=.
+      iApply (sim_tgt_expr_bind [CallCtx _ [] _] (_ @ -) with "[-]") => /=.
+      iApply sim_tgt_rec_BinOp; [done|]. iModIntro => /=.
+      iApply (sim_tgt_expr_bind [CallCtx _ [_] _] (_ @ -) with "[-]") => /=.
+      iApply sim_tgt_rec_BinOp; [done|]. iModIntro => /=.
+      iApply (sim_tgt_expr_bind [CallCtx _ [_; _] _] (_ @ -) with "[-]") => /=.
+      iApply sim_tgt_rec_BinOp; [done|]. iModIntro => /=.
+      destruct (decide (d.1 = s.1 ∧ s.2 ≤ d.2 + length hvss)) as [[??]|Hn]; simplify_eq.
+      + rewrite -(insert_union_l _ _ s) insert_union_r. 2: { apply array_lookup_None => /=. lia. }
+        rewrite delete_union. rewrite delete_notin. 2: { apply array_lookup_None => /=. lia. }
+        destruct (decide (d = s)); simplify_eq.
+        * rewrite delete_insert_delete delete_insert. 2: { apply array_lookup_None => /=. lia. }
+          iApply ("IH" with "[%] [%] [//] [//] [%] Hm"). { lia. } { done. } { simpl. lia. }
+          iIntros "?". iSplit!. iApply ("HΦ" with "[-]").
+          rewrite -insert_union_l -insert_union_r. 2: { apply array_lookup_None => /=. lia. }
+          rewrite insert_insert. by iApply (big_sepM_insert_2 with "[Hdv]"); [done|].
+        * rewrite delete_insert_ne // delete_insert. 2: { apply array_lookup_None => /=. lia. }
+          have ?: d.2 ≠ s.2. { destruct d, s; naive_solver. }
+          rewrite (array_insert s ( d+ₗ1)) //=; [|lia].
+          iApply ("IH" with "[%] [%] [//] [//] [%] Hm"). { lia. } { rewrite insert_length. done. } { simpl. lia. }
+          iIntros "?". iSplit!. iApply ("HΦ" with "[-]").
+          rewrite -insert_union_l. iApply (big_sepM_insert_2 with "[Hdv]"); [done|].
+          admit.
+      + rewrite delete_union delete_insert. 2: { apply array_lookup_None => /=. lia. }
+        rewrite delete_insert_ne. 2: { move => ?. subst. lia. }
+        rewrite delete_notin. 2: { apply array_lookup_None => /=. lia. }
+        rewrite -!insert_union_l (big_sepM_delete _ (<[s:=_]>_) s v). 2: by simplify_map_eq.
+        iDestruct "Hm" as "[Hsv Hm]".
+        rewrite delete_insert. 2: { apply lookup_union_None. rewrite !array_lookup_None => /=. lia. }
+        iApply ("IH" with "[%] [%] [//] [//] [%] Hm"). { lia. } { done. } { simpl. lia. }
+        iIntros "?". iSplit!. iApply ("HΦ" with "[-]").
+        rewrite -insert_union_r. 2: { apply array_lookup_None => /=. lia. }
+        iApply (big_sepM_insert_2 with "[Hdv]"); [done|].
+        iApply (big_sepM_insert_2 with "[Hsv]"); [done|].
+        done.
+    - destruct hvss as [|v hvss _] using rev_ind; [done|] => /=.
+      destruct hvsd as [|vd hvsd _] using rev_ind; [simplify_eq/=; lia|] => /=.
+      rewrite app_length/=. rewrite !app_length/= in Hlen.
+      have -> : (- (length hvss + 1)%nat + 1) = - Z.of_nat (length hvss) by lia.
+      rewrite !array_app /= !array_cons !array_nil.
+      have -> : s +ₗ - length hvss +ₗ length hvss = s by apply loc_eq; split!; lia.
+      have -> : d +ₗ - length hvss +ₗ length hvss = d by apply loc_eq; split!; lia.
+      have -> : d +ₗ - length hvss +ₗ length hvsd = d by apply loc_eq; split!; lia.
+      rewrite -insert_union_r. 2: { apply array_lookup_None => /=. lia. }
+      rewrite -insert_union_r. 2: { apply array_lookup_None => /=. lia. }
+      rewrite !right_id_L.
+      iDestruct (big_sepM_lookup_acc _ _ s v with "[$]") as "[Hsv Hm]". { by simplify_map_eq. }
+      iApply (sim_tgt_rec_Load with "Hsv"). iIntros "Hsv !>" => /=.
+      iDestruct ("Hm" with "[$]") as "Hm".
+      have [? Hx]: is_Some ((<[s:=v]> (array (s +ₗ - length hvss) hvss) ∪ <[d:=vd]> (array (d +ₗ - length hvss) hvsd)) !! d).
+      { apply lookup_union_is_Some. simplify_map_eq. naive_solver. }
+      rewrite (big_sepM_delete _ _ _ _ Hx).
+      iDestruct "Hm" as "[Hdv Hm]".
+      iApply (sim_tgt_rec_Store with "Hdv"). iIntros "Hdv !>" => /=.
+      iApply (sim_tgt_rec_LetE). iIntros "!>" => /=.
+      iApply (sim_tgt_expr_bind [CallCtx _ [] _] (_ @ -) with "[-]") => /=.
+      iApply sim_tgt_rec_BinOp; [done|]. iModIntro => /=.
+      iApply (sim_tgt_expr_bind [CallCtx _ [_] _] (_ @ -) with "[-]") => /=.
+      iApply sim_tgt_rec_BinOp; [done|]. iModIntro => /=.
+      iApply (sim_tgt_expr_bind [CallCtx _ [_; _] _] (_ @ -) with "[-]") => /=.
+      iApply sim_tgt_rec_BinOp; [done|]. iModIntro => /=.
+      destruct (decide (d.1 = s.1 ∧ d.2 ≤ s.2 + length hvss)) as [[??]|Hn]; simplify_eq.
+      + rewrite -(insert_union_l _ _ s) insert_union_r. 2: { apply array_lookup_None => /=. lia. }
+        rewrite delete_union. rewrite delete_notin. 2: { apply array_lookup_None => /=. lia. }
+        destruct (decide (d = s)); simplify_eq.
+        * rewrite delete_insert_delete delete_insert. 2: { apply array_lookup_None => /=. lia. }
+          iApply ("IH" with "[%] [%] [%] [%] [%] Hm"). { lia. } { lia. }
+          { apply loc_eq; split!; lia. } { apply loc_eq; split!; lia. } { simpl. lia. }
+          iIntros "?". iSplit!. iApply ("HΦ" with "[-]").
+          rewrite -(insert_union_r _ ∅). 2: { apply array_lookup_None => /=. lia. }
+          rewrite -insert_union_l right_id_L -insert_union_r. 2: { apply array_lookup_None => /=. lia. }
+          rewrite insert_insert. by iApply (big_sepM_insert_2 with "[Hdv]"); [done|].
+        * rewrite delete_insert_ne // delete_insert. 2: { apply array_lookup_None => /=. lia. }
+          have ?: d.2 ≠ s.2. { destruct d, s; naive_solver. }
+          rewrite (array_insert s (d +ₗ - length hvss)) //=; [|lia].
+          iApply ("IH" with "[%] [%] [%] [%] [%] Hm"). { lia. } { rewrite insert_length. lia. }
+          { apply loc_eq; split!; lia. } { apply loc_eq; split!; lia. } { simpl. lia. }
+          iIntros "?". iSplit!. iApply ("HΦ" with "[-]").
+          rewrite -(insert_union_r _ ∅). 2: { apply array_lookup_None => /=. lia. }
+          rewrite right_id_L -insert_union_l. iApply (big_sepM_insert_2 with "[Hdv]"); [done|].
+          admit.
+      + rewrite delete_union delete_insert. 2: { apply array_lookup_None => /=. lia. }
+        rewrite delete_insert_ne. 2: { move => ?. subst. lia. }
+        rewrite delete_notin. 2: { apply array_lookup_None => /=. lia. }
+        rewrite -!insert_union_l (big_sepM_delete _ (<[s:=_]>_) s v). 2: by simplify_map_eq.
+        iDestruct "Hm" as "[Hsv Hm]".
+        rewrite delete_insert. 2: { apply lookup_union_None. rewrite !array_lookup_None => /=. lia. }
+        iApply ("IH" $! hvss hvsd with "[%] [%] [%] [%] [%] Hm"). { lia. } { lia. }
+        { apply loc_eq; split!; lia. } { apply loc_eq; split!; lia. } { simpl. lia. }
+        iIntros "?". iSplit!. iApply ("HΦ" with "[-]").
+        rewrite -(insert_union_r _ _ d). 2: { apply array_lookup_None => /=. lia. }
+        rewrite -insert_union_l right_id_L -insert_union_r. 2: { apply array_lookup_None => /=. lia. }
+        iApply (big_sepM_insert_2 with "[Hdv]"); [done|].
+        iApply (big_sepM_insert_2 with "[Hsv]"); [done|].
+        done.
   Admitted.
 
-  Lemma sim_memmove Π Φ d s n hvs :
-    n = Z.of_nat (length hvs) →
+  Lemma sim_memmove hvss hvsd Π Φ d s n :
+    n = Z.of_nat (length hvss) →
+    length hvss = length hvsd →
     "memmove" ↪ Some memmove_rec -∗
     "memcpy" ↪ Some memcpy_rec -∗
     □ (∀ l1 l2 Φ,
         (∀ b, ⌜l1.1 = l2.1 → b = bool_decide (l1.2 ≤ l2.2)⌝ -∗ Φ (Val (ValBool b) @ -) Π) -∗
           TGT Call "locle" [Val (ValLoc l1); Val $ ValLoc l2] @ - [{ Π }] {{ Φ }}) -∗
-    ([∗ list] i↦v∈hvs, (s +ₗ i) ↦ v) -∗
-    ([∗ list] i↦_∈hvs, ∃ v, (d +ₗ i) ↦ v) -∗
-    (([∗ list] i↦v∈hvs, (s +ₗ i) ↦ v) -∗ ([∗ list] i↦v∈hvs, (d +ₗ i) ↦ v) -∗ Φ (Val 0 @ -) Π) -∗
+    ([∗ map] l↦v∈array s hvss ∪ array d hvsd, l ↦ v) -∗
+    (([∗ map] l↦v∈array d hvss ∪ array s hvss, l ↦ v) -∗ Φ (Val 0 @ -) Π) -∗
     TGT Call "memmove" [Val (ValLoc d); Val $ ValLoc s; Val $ ValNum n] @ - [{ Π }] {{ Φ }}.
   Proof.
-    iIntros (->) "#Hmemmove #Hmemcpy #Hlocle Hs Hd HΦ".
+    iIntros (-> ?) "#Hmemmove #Hmemcpy #Hlocle Hs HΦ".
     iApply (sim_tgt_expr_bind [] (_ @ -)).
     iApply (sim_tgt_rec_Call_internal with "Hmemmove"); [done|]. iModIntro => /=.
     iApply sim_tgt_rec_AllocA; [econs|] => /=. iIntros (?) "?". destruct ls => //. iModIntro.
     iApply (sim_tgt_expr_bind [IfCtx _ _] (_ @ -) with "[-]") => /=.
     iApply "Hlocle". iIntros (b Hb) => /=.
     iApply sim_tgt_rec_If. iModIntro => /=. destruct b.
-    - iApply (sim_memcpy with "[//] Hs Hd"). { done. } { by left. } { by rewrite bool_decide_true. }
+    - iApply (sim_memcpy with "[//] Hs"). { done. } { done. } { by left. } { by rewrite bool_decide_true. }
       { by rewrite bool_decide_true. } {
         rewrite bool_decide_true // => /Hb Hx. symmetry in Hx. by rewrite bool_decide_eq_true in Hx.
       }
-      iIntros "? ?". iSplit!. iApply sim_tgt_expr_stop2. iApply ("HΦ" with "[$] [$]").
+      iIntros "?". iSplit!. iApply sim_tgt_expr_stop2. iApply ("HΦ" with "[$]").
     - iApply (sim_tgt_expr_bind [CallCtx _ [] _] (_ @ -) with "[-]") => /=.
       iApply (sim_tgt_expr_bind [BinOpRCtx _ _] (_ @ -) with "[-]") => /=.
       iApply sim_tgt_rec_BinOp; [done|]. iModIntro => /=.
@@ -326,210 +958,61 @@ Section memmove.
       iApply (sim_tgt_expr_bind [BinOpRCtx _ _] (_ @ -) with "[-]") => /=.
       iApply sim_tgt_rec_BinOp; [done|]. iModIntro => /=.
       iApply sim_tgt_rec_BinOp; [done|]. iModIntro => /=.
-      iApply (sim_memcpy with "[//] Hs Hd"). { done. } { by right. }
+      iApply (sim_memcpy with "[//] Hs"). { done. } { done. } { by right. }
       { rewrite bool_decide_false; [|done]. rewrite offset_loc_assoc.
-        have -> : (length hvs + -1 + (- length hvs + 1)) = 0 by lia.
+        have -> : (length hvss + -1 + (- length hvss + 1)) = 0 by lia.
         rewrite offset_loc_0. done. }
       { rewrite bool_decide_false; [|done]. rewrite offset_loc_assoc.
-        have -> : (length hvs + -1 + (- length hvs + 1)) = 0 by lia.
+        have -> : (length hvss + -1 + (- length hvss + 1)) = 0 by lia.
         rewrite offset_loc_0. done. } {
         rewrite bool_decide_false // => /Hb Hx. symmetry in Hx. rewrite bool_decide_eq_false in Hx.
         simpl. lia.
       }
-      iIntros "? ?". iSplit!. iApply sim_tgt_expr_stop2. iApply ("HΦ" with "[$] [$]").
+      iIntros "?". iSplit!. iApply sim_tgt_expr_stop2. iApply ("HΦ" with "[$]").
   Qed.
 
-  Lemma sim_locle Π Φ l1 l2 :
+  Local Canonical Structure spec_mod_lang_unit.
+  Lemma sim_locle s fns fns1 Φ l1 l2 Π_s :
+    (∀ P, P (λ σ', σ' ≈{rec_link_trans fns1 {["locle"]} _ _}≈>ₜ Π_s) -∗ Π_s None P) →
+    let Π := λ κ P, (∀ σl, (σl ⤇ₜ λ Π, TGT locle_spec [{Π}] {{_, _, False}}) -∗
+              link_tgt_left_handler (rec_link_filter fns1 {["locle"]}) Π_s s σl κ P)%I in
+    rec_fn_auth fns -∗
+    "locle" ↪ None -∗
     (∀ b, ⌜l1.1 = l2.1 → b = bool_decide (l1.2 ≤ l2.2)⌝ -∗ Φ (Val (ValBool b) @ -) Π) -∗
     TGT Call "locle" [Val (ValLoc l1); Val $ ValLoc l2] @ - [{ Π }] {{ Φ }}.
-  Proof. Admitted.
-
+  Proof.
+    iIntros (HΠ_s Π) "#Hfns #Hf HΦ".
+    iApply (sim_tgt_rec_Call_external with "[$]"). iIntros (?) "!>". iIntros (σl) "Hσl".
+    iIntros (??????). destruct!/=. case_bool_decide => //. rewrite (bool_decide_true (_ ∈ _)) //.
+    iApply HΠ_s. iIntros (σ') "Hσ'".
+    iApply (sim_tgt_link_right_recv with "[-]"). iApply "Hσl".
+    rewrite /locle_spec unfold_forever -/locle_spec.
+    rewrite /TReceive bind_bind bind_bind.
+    iApply (sim_tgt_TExist with "[-]"). iIntros ([[??]?]) "!>".
+    rewrite bind_bind. setoid_rewrite bind_ret_l.
+    iApply (sim_tgt_TVis with "[-]"). iIntros "!>" (?). simplify_eq/=.
+    iApply HΠ_s. iIntros (?) "Hσl".
+    iApply (sim_tgt_link_right with "[-]"). iApply "Hσl".
+    rewrite bind_bind. iApply (sim_tgt_TAssume with "[-]"); [done|]. iIntros "!>".
+    rewrite bind_bind. iApply (sim_tgt_TAll with "[-]"). iIntros "!>".
+    rewrite bind_bind. iApply (sim_tgt_TAll with "[-]"). iIntros "!>".
+    rewrite bind_bind. iApply (sim_tgt_TAssume with "[-]"); [done|]. iIntros "!>".
+    rewrite bind_bind. iApply (sim_tgt_TExist with "[-]"). iIntros (b) "!>".
+    rewrite bind_bind. iApply (sim_tgt_TAssert with "[-]"). iIntros (?) "!>".
+    iApply (sim_tgt_TVis with "[-]"). iIntros "!>" (??????). destruct!/=.
+    iApply HΠ_s. iIntros (?) "Hσl".
+    iApply (sim_tgt_link_left_recv with "[-]"). iApply "Hσ'".
+    iApply (sim_tgt_rec_Waiting with "[$]"). iIntros "??".
+    iSplit. { iIntros. iModIntro. iIntros. simplify_eq. }
+    iIntros (???) "!>". iIntros (?). simplify_eq.
+    iApply HΠ_s. iIntros (?) "Hσ'".
+    iApply (sim_tgt_link_left with "[-]"). iApply ("Hσ'" with "[$] [$]").
+    iApply (sim_tgt_expr_wand1 with "[HΦ]").
+    { iApply sim_tgt_expr_stop2. by iApply "HΦ". }
+    iIntros (??) "HΠ". by iApply "HΠ".
+  Qed.
 
 End memmove.
-
-Section sim.
-  Context {Σ : gFunctors} {EV : Type} `{!dimsumGS Σ}.
-
-  Definition sim_tgt_handler {m_t m_s : mod_trans EV}
-    (σ : m_state m_s) :
-    option EV → ((m_state m_t → iProp Σ) → iProp Σ) → iProp Σ :=
-    λ κ Pσ, (σ ≈{m_s}≈>ₛ (λ κ' σ_s', ⌜κ = κ'⌝ ∗ Pσ (λ σ_t', σ_t' ⪯{m_t, m_s} σ_s')))%I.
-
-  Lemma sim_tgt_handler_intro m_t m_s σ_t σ_s :
-    σ_t ≈{m_t}≈>ₜ sim_tgt_handler σ_s -∗ σ_t ⪯{m_t, m_s} σ_s.
-  Proof.
-    iIntros "?". rewrite sim_unfold.
-    iApply (sim_tgt_wand with "[$]"). iIntros (??) "?".
-    iApply (sim_src_wand with "[$]"). iIntros (??) "[% ?]".
-    iSplit; [done|]. by iApply bi_mono1_intro0.
-  Qed.
-
-End sim.
-
-Section link.
-  Context {Σ : gFunctors} {EV : Type} {S : Type} `{!dimsumGS Σ}.
-  Implicit Types (R : seq_product_case → S → EV → seq_product_case → S → EV → bool → Prop).
-
-  Lemma sim_tgt_link_None R m1 m2 s σ1 σ2 Π :
-    ▷ₒ (∀ e p' s' e' ok,
-        ⌜R SPNone s e p' s' e' ok⌝ -∗
-        Π (Some (Incoming, e')) (λ P, P (link_to_case ok p' e', s', σ1, σ2))) -∗
-    (MLFNone, s, σ1, σ2) ≈{link_trans R m1 m2}≈>ₜ Π.
-  Proof.
-    iIntros "HΠ".
-    iApply (sim_tgt_bi_mono1 with "[-]").
-    iApply sim_tgt_state_transform; [done|] => /=.
-    iApply (sim_tgt_map with "[-]").
-    iApply sim_tgt_seq_product_None. iIntros (p) "!>". iIntros (????).
-    inv_all @link_filter.
-    iApply (bi_mono1_intro with "[HΠ]"); [by iApply "HΠ"|] => /=.
-    iIntros (?) "?". iIntros ([[[??]?]?] ?); simplify_eq/=. by repeat case_match; simplify_eq/=.
-  Qed.
-
-  Definition link_tgt_left_handler R {m1 m2 : mod_trans (io_event EV)}
-    (Π : option (io_event EV) → ((link_case EV * S * m_state m1 * m_state m2 → iProp Σ) → iProp Σ) → iProp Σ)
-    (s : S) (σ2 : m_state m2)
-    : option (io_event EV) → ((m_state m1 → iProp Σ) → iProp Σ) → iProp Σ :=
-    λ κ Pσ,
-      match κ with
-            | None => Π None (λ P, Pσ (λ σ1', P (MLFLeft, s, σ1', σ2)))
-            | Some e => ∀ p' s' e' ok, ⌜R SPLeft s e.2 p' s' e' ok⌝ -∗ ⌜e.1 = Outgoing⌝ -∗
-                 Π (if p' is SPNone then Some (Outgoing, e') else None)
-                 (λ P, Pσ (λ σ1', P (link_to_case ok p' e', s', σ1', σ2)))
-            end%I.
-
-  Lemma sim_tgt_link_left R m1 m2 s σ1 σ2 Π :
-    σ1 ≈{m1}≈>ₜ link_tgt_left_handler R Π s σ2 -∗
-    (MLFLeft, s, σ1, σ2) ≈{link_trans R m1 m2}≈>ₜ Π.
-  Proof.
-    iIntros "Hsim".
-    iApply (sim_tgt_bi_mono1 with "[-]").
-    iApply sim_tgt_state_transform; [done|] => /=.
-    iApply (sim_tgt_map with "[-]").
-    iApply sim_tgt_seq_product_left.
-    iApply (sim_tgt_bi_mono2 with "[-]").
-    iApply (sim_tgt_wand with "Hsim").
-    iIntros (κ ?) "Hsim". iIntros (??????). destruct κ; destruct!/=.
-    - inv_all @link_filter.
-      iApply (bi_mono1_intro with "[Hsim]"); [by iApply "Hsim"|].
-      iIntros (?) "HP". iApply (bi_mono1_intro with "HP").
-      iIntros (?) "?". iIntros ([[[??]?]?]?). simplify_eq/=. by repeat case_match; simplify_eq/=.
-    - iApply (bi_mono1_intro with "[Hsim]"); [by iApply "Hsim"|].
-      iIntros (?) "HP". iApply (bi_mono1_intro with "HP").
-      iIntros (?) "?". iIntros ([[[??]?]?]?). simplify_eq/=. done.
-  Qed.
-
-  Lemma sim_tgt_link_left_recv R m1 m2 s σ1 σ2 Π e :
-    (σ1 ≈{m1}≈>ₜ λ κ Pσ,
-      match κ with
-      | None => Π None (λ P, Pσ (λ σ1', P (MLFRecvL e, s, σ1', σ2)))
-      | Some e' => ⌜e' = (Incoming, e)⌝ -∗ Π None (λ P, Pσ (λ σ1', P (MLFLeft, s, σ1', σ2)))
-      end%I) -∗
-    (MLFRecvL e, s, σ1, σ2) ≈{link_trans R m1 m2}≈>ₜ Π.
-  Proof.
-    iIntros "Hsim".
-    iApply (sim_tgt_bi_mono1 with "[-]").
-    iApply sim_tgt_state_transform; [done|] => /=.
-    iApply (sim_tgt_map with "[-]").
-    iApply sim_tgt_seq_product_left.
-    iApply (sim_tgt_bi_mono2 with "[-]").
-    iApply (sim_tgt_wand with "Hsim").
-    iIntros (κ ?) "Hsim". iIntros (??????). destruct κ; destruct!/=.
-    - inv_all @link_filter.
-      iApply (bi_mono1_intro with "[Hsim]"); [by iApply "Hsim"|].
-      iIntros (?) "HP". iApply (bi_mono1_intro with "HP").
-      iIntros (?) "?". iIntros ([[[??]?]?]?). by simplify_eq/=.
-    - iApply (bi_mono1_intro with "[Hsim]"); [by iApply "Hsim"|].
-      iIntros (?) "HP". iApply (bi_mono1_intro with "HP").
-      iIntros (?) "?". iIntros ([[[??]?]?]?). simplify_eq/=. done.
-  Qed.
-End link.
-
-Program Definition spec_mod_lang {Σ} (EV S : Type) (state_interp : S → iProp Σ)  : mod_lang EV Σ := {|
-  mexpr := spec EV S void;
-  mectx := unit;
-  mfill _ := id;
-  mcomp_ectx _ _:= tt;
-  mtrans := spec_trans EV S;
-  mexpr_rel σ t := σ.1 ≡ t;
-  mstate_interp σ := state_interp σ.2;
-|}.
-Next Obligation. done. Qed.
-
-Definition spec_mod_lang_unit {Σ} (EV : Type) : mod_lang EV Σ :=
-  spec_mod_lang EV unit (λ _, True%I).
-
-Section spec.
-  Context `{!dimsumGS Σ} {EV S : Type} {state_interp : S → iProp Σ}.
-
-  Global Instance sim_src_expr_spec_proper :
-    Proper ((≡) ==> (=) ==> (=) ==> (⊣⊢)) (sim_src_expr (Λ:=spec_mod_lang EV S state_interp)).
-  Proof.
-    move => ?? ? ?? -> ?? ->.
-    Local Transparent sim_src_expr.
-    Local Typeclasses Transparent sim_src_expr.
-    iSplit; iIntros "HP" (?) "?"; iIntros (??); simplify_eq/=; iApply ("HP" with "[$]"); iPureIntro => /=.
-    all: by etrans; [done|].
-    Unshelve. all: exact tt.
-  Qed.
-
-  Let X := (spec_mod_lang EV _ state_interp).
-  Local Canonical Structure X.
-
-  Lemma sim_src_TAll {T} k Π Φ :
-    (∀ x, SRC (k x) [{ Π }] {{ Φ }}) -∗
-    SRC (Spec.bind (TAll T) k) [{ Π }] {{ Φ }}.
-  Proof.
-    iIntros "Hsim". rewrite unfold_bind/=. setoid_rewrite unfold_bind; simpl.
-    iApply sim_src_expr_step_None. iIntros (?[??]?) "?". simplify_eq/=. iModIntro.
-    iExists _. iSplit. { iPureIntro. by econs. }
-    iIntros ([??] [??]) "!>". simplify_eq. iSplit!. iFrame. iApply "Hsim".
-  Qed.
-
-  Lemma sim_src_TExist {T} x k Π Φ :
-    SRC (k x) [{ Π }] {{ Φ }} -∗
-    SRC (Spec.bind (TExist T) k) [{ Π }] {{ Φ }}.
-  Proof.
-    iIntros "Hsim". rewrite unfold_bind/=. setoid_rewrite unfold_bind; simpl.
-    iApply sim_src_expr_step_None. iIntros (?[??]?) "?". simplify_eq/=. iModIntro.
-    iExists _. iSplit. { iPureIntro. by econs. }
-    iIntros ([??] ?) "!>". simplify_eq. iSplit!. iFrame.
-  Qed.
-
-  Lemma sim_src_TAssume k Π Φ P :
-    (⌜P⌝ -∗ SRC (k tt) [{ Π }] {{ Φ }}) -∗
-    SRC (Spec.bind (TAssume P) k) [{ Π }] {{ Φ }}.
-  Proof.
-    iIntros "Hsim". rewrite unfold_bind/=. setoid_rewrite unfold_bind; simpl.
-    iApply sim_src_expr_step_None. iIntros (?[??]?) "?". simplify_eq/=. iModIntro.
-    iExists _. iSplit. { iPureIntro. by econs. }
-    iIntros ([??] [??]) "!>". simplify_eq. iSplit!. iFrame. by iApply "Hsim".
-  Qed.
-
-  Lemma sim_src_TAssert k Π Φ (P : Prop) :
-    P →
-    SRC (k tt) [{ Π }] {{ Φ }} -∗
-    SRC (Spec.bind (TAssert P) k) [{ Π }] {{ Φ }}.
-  Proof.
-    iIntros (?) "Hsim". rewrite unfold_bind/=. setoid_rewrite unfold_bind; simpl.
-    iApply sim_src_expr_step_None. iIntros (?[??]?) "?". simplify_eq/=. iModIntro.
-    iExists _. iSplit. { iPureIntro. by econs. }
-    iIntros ([??] ?) "!>". simplify_eq. iSplit!. iFrame.
-    Unshelve. done.
-  Qed.
-
-  Lemma sim_src_TVis k Π Φ e :
-    (∀ σ, σ ⤇ₛ (λ Π, SRC k tt [{ Π }] {{ Φ }}) -∗ Π (Some e) σ) -∗
-    SRC (Spec.bind (TVis e) k) [{ Π }] {{ Φ }}.
-  Proof.
-    iIntros "Hsim". rewrite unfold_bind/=. setoid_rewrite unfold_bind; simpl.
-    iApply sim_src_expr_step. iIntros (?[??]?) "?". simplify_eq/=. iModIntro.
-    iExists _, _. iSplit. { iPureIntro. by econs. }
-    iIntros ([??] ?) "!> HΦ". simplify_eq.
-    iApply "Hsim". iIntros (?) "?". by iApply ("HΦ" with "[//] [$]").
-  Qed.
-End spec.
-
 
 Section memmove.
   Context `{!dimsumGS Σ} `{!recGS Σ}.
@@ -552,19 +1035,21 @@ Section memmove.
     iApply (sim_src_TExist (_, _, _)).
     rewrite bind_bind. setoid_rewrite bind_ret_l.
     iApply sim_src_TVis. iIntros (?) "Hsrc". iSplit!.
+    iApply bi_mono1_intro0.
     iApply (sim_tgt_handler_intro with "[-]"). iApply sim_tgt_stop.
     iApply "Hsrc".
     iApply sim_src_TAssume. iIntros (?).
     iApply sim_src_TAssume. iIntros (?). simplify_eq.
     rewrite bool_decide_true; [|done].
     iApply sim_src_expr_stop1. iIntros (?) "Hsrc". iSplit!.
+    iApply bi_mono1_intro0.
     iApply (sim_tgt_handler_intro with "[-]").
     iApply (sim_tgt_link_left_recv with "[-]").
     iApply (sim_tgt_expr_elim [] (_ @ _) with "[Ha Hh] [-]"); [done| by iFrame |] => /=.
     iApply (sim_tgt_rec_Waiting with "[$]"). iIntros "Hh Ha".
     iSplit; [|by iIntros].
     iIntros (???? Hin) "!>". iIntros (?). simplify_map_eq.
-    iApply sim_src_stop. iSplit!. iIntros (?) "Htgt".
+    iApply sim_src_stop. iSplit!. iApply bi_mono1_intro0. iIntros (?) "Htgt".
     iApply (sim_tgt_handler_intro with "[-]").
     iApply (sim_tgt_link_left with "[-]").
     iApply ("Htgt" with "[Hh] [Ha]"). admit. admit.
@@ -578,6 +1063,117 @@ Section memmove.
     iApply (sim_tgt_expr_bind [LetECtx _ _] (_ @ -) with "[-]") => /=.
     iApply (sim_tgt_expr_bind [StoreLCtx _] (_ @ -) with "[-]") => /=.
     iApply sim_tgt_rec_BinOp; [done|]. iModIntro => /=.
+    iApply (sim_tgt_rec_Store with "Hl0"). iIntros "Hl0 !>" => /=.
+    iApply sim_tgt_rec_LetE. iIntros "!>" => /=.
+    iApply (sim_tgt_expr_bind [LetECtx _ _] (_ @ -) with "[-]") => /=.
+    iApply (sim_tgt_expr_bind [StoreLCtx _] (_ @ -) with "[-]") => /=.
+    iApply sim_tgt_rec_BinOp; [done|]. iModIntro => /=.
+    iApply (sim_tgt_rec_Store with "Hl1"). iIntros "Hl1 !>" => /=.
+    iApply sim_tgt_rec_LetE. iIntros "!>" => /=.
+    iApply (sim_tgt_expr_bind [LetECtx _ _] (_ @ -) with "[-]") => /=.
+    iApply (sim_tgt_expr_bind [CallCtx _ [] _] (_ @ -) with "[-]") => /=.
+    iApply sim_tgt_rec_BinOp; [done|]. iModIntro => /=.
+    iApply (sim_tgt_expr_bind [CallCtx _ [_] _] (_ @ -) with "[-]") => /=.
+    iApply sim_tgt_rec_BinOp; [done|]. iModIntro => /=.
+    iApply (sim_tgt_expr_wand1 with "[-]"). 2: shelve.
+    iApply (sim_memmove [ValNum 1; ValNum 2] [ValNum 2; ValNum 0] with "[] [] [] [Hl0 Hl1 Hl2]").
+    { done. } { done. }
+    { by iApply (rec_fn_intro with "[$]"). }
+    { by iApply (rec_fn_intro with "[$]"). }
+    { iIntros "!>" (???) "HΦ".
+      iApply sim_locle. 2: done. 2: { by iApply (rec_fn_intro with "[$]"). } 2: done.
+      Unshelve. all: shelve_unifiable. 2: exact tt. 2: {
+        iIntros (??) "HΦ". iApply "HΦ". iIntros (?) "?".
+        by iApply (sim_tgt_expr_elim with "[] [-]"); [simpl; done..|].
+      }
+      iIntros (?) "HP". unfold sim_tgt_handler.
+      iApply (sim_src_stop with "[-]"). iSplit!.
+      iApply (bi_mono1_intro with "HP"). iIntros (?) "?".
+      by iApply (sim_tgt_handler_intro with "[-]").
+    }
+    { rewrite !array_cons !array_nil -!insert_union_l !left_id_L.
+      rewrite !offset_loc_assoc insert_insert.
+      iApply (big_sepM_insert_2 with "[Hl0]"); [done|].
+      iApply (big_sepM_insert_2 with "[Hl1]"); [done|].
+      iApply (big_sepM_insert_2 with "[Hl2]"); [done|].
+      done. }
+      iIntros "Hl" => /=. rewrite !array_cons !array_nil -!insert_union_l !left_id_L.
+      rewrite !offset_loc_assoc.
+      rewrite (big_sepM_delete _ _ (l +ₗ 1)). 2: { by simplify_map_eq. }
+      rewrite delete_insert_delete.
+      rewrite delete_insert_ne //. 2: admit.
+      rewrite delete_insert_ne //. 2: admit.
+      rewrite delete_insert //.
+      rewrite big_sepM_insert. 2: admit.
+      rewrite big_sepM_insert. 2: done.
+      iDestruct "Hl" as "[Hl1 [Hl2 [Hl0 _]]]".
+      iApply sim_tgt_rec_LetE. iModIntro => /=.
+      iApply (sim_tgt_expr_bind [LetECtx _ _] (_ @ -) with "[-]") => /=.
+      iApply (sim_tgt_expr_bind [CallCtx _ [] _] (_ @ -) with "[-]") => /=.
+      iApply (sim_tgt_expr_bind [LoadCtx] (_ @ -) with "[-]") => /=.
+      iApply sim_tgt_rec_BinOp; [done|]. iModIntro => /=.
+      iApply (sim_tgt_rec_Load with "Hl1"). iIntros "Hl1 !>" => /=.
+      iApply (sim_tgt_rec_Call_external). { by iApply (rec_fn_intro with "[$]"). }
+      iIntros (?) "!>". iIntros (σ') "Hlocle".
+      iIntros (??????). destruct!/=. rewrite bool_decide_false//.
+      iApply "Hsrc". iApply sim_src_TExist. iApply sim_src_TVis.
+      iIntros (?) "Hsrc". iSplit!. iApply bi_mono1_intro0.
+      iIntros (?) "Htgt". iApply (sim_tgt_handler_intro with "[-]").
+      iApply (sim_tgt_link_None with "[-]"). iIntros "!>" (??????). destruct!/=.
+      iApply "Hsrc". iApply sim_src_TExist. iApply sim_src_TVis.
+      iIntros (?) "Hsrc". iSplit!. iApply bi_mono1_intro0.
+      iApply (sim_tgt_handler_intro with "[-]"). iApply sim_tgt_stop.
+      iApply "Hsrc". iApply sim_src_TAssume. iIntros (?). iApply sim_src_expr_stop1.
+      iIntros (?) "Hsrc". iSplit!. iApply bi_mono1_intro0. case_match; destruct!/=.
+      iApply (sim_tgt_handler_intro with "[-]").
+      iApply (sim_tgt_link_left_recv with "[-]").
+      iApply "Htgt".
+      iApply (sim_tgt_rec_Waiting with "[$]"). iIntros "Hh Ha".
+      iSplit; [iIntros; iModIntro; by iIntros|].
+      iIntros (???) "!>". iIntros (?). simplify_eq.
+      iApply sim_src_stop. iSplit!. iApply bi_mono1_intro0.
+      iIntros (?) "Htgt".
+      iApply (sim_tgt_handler_intro with "[-]").
+      iApply (sim_tgt_link_left with "[-]").
+      iApply ("Htgt" with "[$] [$]").
+      iApply sim_tgt_expr_stop2 => /=.
+      iApply (sim_tgt_rec_LetE with "[-]"). iIntros "!>" => /=.
+      iApply (sim_tgt_expr_bind [LetECtx _ _] (_ @ -) with "[-]") => /=.
+      iApply (sim_tgt_expr_bind [CallCtx _ [] _] (_ @ -) with "[-]") => /=.
+      iApply (sim_tgt_expr_bind [LoadCtx] (_ @ -) with "[-]") => /=.
+      iApply sim_tgt_rec_BinOp; [done|]. iModIntro => /=.
+      iApply (sim_tgt_rec_Load with "Hl2"). iIntros "Hl2 !>" => /=.
+      iApply (sim_tgt_rec_Call_external). { by iApply (rec_fn_intro with "[$]"). }
+      iIntros (?) "!>". iIntros (??????). destruct!/=. rewrite bool_decide_false//.
+      iApply "Hsrc". iApply sim_src_TExist. iApply sim_src_TVis.
+      iIntros (?) "Hsrc". iSplit!. iApply bi_mono1_intro0.
+      iIntros (?) "Htgt". iApply (sim_tgt_handler_intro with "[-]").
+      iApply (sim_tgt_link_None with "[-]"). iIntros "!>" (??????). destruct!/=.
+      iApply "Hsrc". iApply sim_src_TExist. iApply sim_src_TVis.
+      iIntros (?) "Hsrc". iSplit!. iApply bi_mono1_intro0.
+      iApply (sim_tgt_handler_intro with "[-]"). iApply sim_tgt_stop.
+      iApply "Hsrc". iApply sim_src_TAssume. iIntros (?). iApply sim_src_expr_stop1.
+      iIntros (?) "Hsrc". iSplit!. iApply bi_mono1_intro0. case_match; destruct!/=.
+      iApply (sim_tgt_handler_intro with "[-]").
+      iApply (sim_tgt_link_left_recv with "[-]").
+      iApply "Htgt".
+      iApply (sim_tgt_rec_Waiting with "[$]"). iIntros "Hh Ha".
+      iSplit; [iIntros; iModIntro; by iIntros|].
+      iIntros (???) "!>". iIntros (?). simplify_eq.
+      iApply sim_src_stop. iSplit!. iApply bi_mono1_intro0.
+      iIntros (?) "Htgt".
+      iApply (sim_tgt_handler_intro with "[-]").
+      iApply (sim_tgt_link_left with "[-]").
+      iApply ("Htgt" with "[$] [$]").
+      iApply sim_tgt_expr_stop2 => /=.
+      iApply (sim_tgt_rec_LetE with "[-]"). iIntros "!>" => /=.
+      iApply sim_tgt_expr_stop2 => /=. iSplit!.
+      iSplitL "Hl0 Hl1 Hl2".
+      { iSplit!. iSplitL "Hl0"; eauto with iFrame. iSplitL "Hl1"; eauto with iFrame. }
+      iApply sim_tgt_rec_ReturnExt. iIntros (?) "!>".
+      iIntros (??????). destruct!/=.
+      iApply "Hsrc". iApply sim_src_TUb_end.
+    Unshelve. exact: tt.
   Admitted.
 End memmove.
 
